experiments: new version of the state monad without allocation list

coq_translation/examples-from-rust-book/MonadExperiments.v
@@ -1,6 +1,7 @@
 (** Experiments for the definition of a Rust monad. *)
 Require Coq.Lists.List.
 Require Import Coq.ZArith.ZArith.
+Require Import CoqOfRust.RecordUpdate.
 
 Global Set Primitive Projections.
 Global Set Printing Projections.
@@ -9,148 +10,151 @@ Global Open Scope Z_scope.
 Import List.ListNotations.
 
 Module State.
-  Class Trait (Self Address : Set) : Type := {
+  Class Trait (State Address : Set) : Type := {
     get_Set : Address -> Set;
-    read (a : Address) : Self -> option (get_Set a);
-    write (a : Address) : Self -> get_Set a -> Self;
+    read (a : Address) : State -> option (get_Set a);
+    write (a : Address) : State -> get_Set a -> State;
   }.
 
   Module Valid.
+    (** A valid state should behave as map from address to optional values
+        of the type given by the address. A value is [None] while not
+        allocated, and [Some] once allocated. It is impossible to free
+        allocated values. *)
     Record t `(T : Trait) : Prop := {
-      same (a : Address) (s : Self) (v : get_Set a) :
+      (* Read after a [write] used as a successful allocation. *)
+      same_alloc (a : Address) (s : State) (v : get_Set a) :
         read a (write a s v) <> None ->
         read a (write a s v) = Some v;
-      different (a1 a2 : Address) (s : Self) (v2 : get_Set a2) :
+      (* Read after a [write] on an already allocated address. *)
+      same_write (a : Address) (s : State) (v : get_Set a) :
+        read a s <> None ->
+        read a (write a s v) = Some v;
+      different (a1 a2 : Address) (s : State) (v2 : get_Set a2) :
         a1 <> a2 ->
         read a1 (write a2 s v2) = read a1 s;
       }.
   End Valid.
 End State.
 
-Module Allocation.
-  Definition t (Address : Set) : Set :=
-    list (option Address).
+Module MutRef.
+  Inductive t `{State.Trait} : Set -> Set :=
+  | Make (a : Address) : t (State.get_Set a).
+End MutRef.
+Definition MutRef `{State.Trait} := MutRef.t.
 
-  Fixpoint get_rev {Address : Set} (allocation : t Address) (index : nat)
-    : option Address :=
-    match index, allocation with
-    | _, [] => None
-    | O, Some address :: _ => Some address
-    | O, None :: _ => None
-    | S index, _ :: allocation => get_rev allocation index
+Module Ref.
+  Inductive t `{State.Trait} (A : Set) : Set :=
+  | Immutable : A -> t A
+  | OfMutRef : MutRef A -> t A.
+  Arguments Immutable {_ _ _ _}.
+  Arguments OfMutRef {_ _ _ _}.
+End Ref.
+Definition Ref `{State.Trait} := Ref.t.
+
+Module RawMonad.
+  Inductive t `{State.Trait} (A : Set) : Set :=
+  | Pure : A -> t A
+  | Bind {B : Set} : t B -> (B -> t A) -> t A
+  | AddressOracle {B : Set} : (MutRef B -> t A) -> t A
+  | Impossible : t A.
+  Arguments Pure {_ _ _ _}.
+  Arguments Bind {_ _ _ _ _}.
+  Arguments AddressOracle {_ _ _ _ _}.
+  Arguments Impossible {_ _ _ _}.
+
+  Definition smart_bind `{State.Trait} {A B : Set} (e1 : t A) (e2 : A -> t B) :
+    t B :=
+    match e1 with
+    | Pure v1 => e2 v1
+    | _ => Bind e1 e2
     end.
+End RawMonad.
+Definition RawMonad `{State.Trait} := RawMonad.t.
 
-  Definition get {Address : Set} (allocation : t Address) (index : nat)
-    : option Address :=
-    get_rev (List.rev allocation) index.
-End Allocation.
-Definition Allocation := Allocation.t.
+Module Run.
+  Inductive t `{State.Trait} {A : Set} : RawMonad A -> A -> Prop :=
+  | Pure (v : A) : t (RawMonad.Pure v) v
+  | Bind {B : Set} (e1 : RawMonad B) (e2 : B -> RawMonad A) (v1 : B) (v2 : A) :
+    t e1 v1 ->
+    t (e2 v1) v2 ->
+    t (RawMonad.Bind e1 e2) v2
+  | AddressOracle {B : Set} (r : MutRef B) (e : MutRef B -> RawMonad A) (v : A) :
+    t (e r) v ->
+    t (RawMonad.AddressOracle e) v.
+End Run.
 
-Module M.
-  Inductive t : Set -> Set :=
-  | Pure {A : Set} : A -> t A
-  | Bind {A B : Set} : t B -> (B -> t A) -> t A
-  | Loop {A : Set} : t A -> (A -> bool) -> t A
-  | Malloc {A : Set} : A -> t nat
-  | Read {A : Set} : nat -> t A
-  | Write {A : Set} : nat -> A -> t unit.
-End M.
-Definition M := M.t.
+Module Exception.
+  Inductive t (R : Set) : Set :=
+  | Return : R -> t R
+  | Continue : t R
+  | Break : t R
+  | Panic {A : Set} : A -> t R.
+  Arguments Return {_}.
+  Arguments Continue {_}.
+  Arguments Break {_}.
+  Arguments Panic {_ _}.
+End Exception.
+Definition Exception := Exception.t.
+
+Definition Monad `{State.Trait} (R A : Set) : Set :=
+  nat -> State -> RawMonad ((A + Exception R) * State).
+
+Definition M `{State.Trait} (A : Set) : Set :=
+  Monad Empty_set A.
+
+Definition pure `{State.Trait} {R A : Set} (v : A) : Monad R A :=
+  fun fuel s => RawMonad.Pure (inl v, s).
+
+Definition bind `{State.Trait} {R A B : Set}
+  (e1 : Monad R A) (e2 : A -> Monad R B) : Monad R B :=
+  fun fuel s =>
+  RawMonad.smart_bind (e1 fuel s) (fun '(v, s) =>
+  match v with
+  | inl v => e2 v fuel s
+  | inr e => RawMonad.Pure (inr e, s)
+  end).
 
 Notation "'let*' x ':=' e1 'in' e2" :=
-  (M.Bind e1 (fun x => e2))
+  (bind e1 (fun x => e2))
   (at level 200, x name, e1 at level 100, e2 at level 200).
 
-Module M_State.
-  Inductive t (Address A : Set) : Set :=
-  | Pure : A -> t Address A
-  | Bind {B : Set} : t Address B -> (B -> t Address A) -> t Address A
-  | GetAddress : (Address -> t Address A) -> t Address A
-  | Cast {B B' : Set} : B -> (B' -> t Address A) -> t Address A
-  | Impossible : t Address A.
-  Arguments Pure {_ _}.
-  Arguments Bind {_ _ _}.
-  Arguments GetAddress {_ _}.
-  Arguments Cast {_ _ _ _}.
-  Arguments Impossible {_ _}.
-End M_State.
-Definition M_State := M_State.t.
-
-Fixpoint run_state {State Address A : Set} `{State.Trait State Address}
-  (fuel : nat) (allocation : Allocation Address) (s : State)
-  (e : M A) {struct fuel} :
-  M_State Address (A * Allocation Address * State) :=
-  match fuel with
-  | O => M_State.Impossible
-  | S fuel =>
-    match e with
-    | M.Pure v =>
-      M_State.Pure (v, allocation, s)
-    | M.Bind e1 e2 =>
-      M_State.Bind
-        (run_state fuel allocation s e1) (fun '(v1, allocation, s) =>
-        run_state fuel allocation s (e2 v1))
-    | M.Loop body is_break as e =>
-      M_State.Bind
-      (run_state fuel allocation s body) (fun '(v, allocation, s) =>
-      if is_break v then
-        M_State.Pure (v, allocation, s)
-      else
-        run_state fuel allocation s e)
-    | M.Malloc v =>
-      M_State.GetAddress (fun address =>
-      (* Check that the address was not yet allocated *)
-      match State.read address s with
-      | None =>
-        let index := List.length allocation in
-        let allocation := Some address :: allocation in
-        M_State.Cast v (fun v =>
-        let s := State.write address s v in
-        (* Check that the address is now allocated *)
-        match State.read address s with
-        | Some _ =>
-          M_State.Pure (index, allocation, s)
-        | None => M_State.Impossible
-        end)
-      | Some _ => M_State.Impossible
-      end)
-    | M.Read index =>
-      match Allocation.get allocation index with
-      | Some address =>
-        match State.read address s with
-        | Some v =>
-          M_State.Cast v (fun v =>
-          M_State.Pure (v, allocation, s))
-        | None => M_State.Impossible
-        end
-      | None => M_State.Impossible
+Definition alloc `{State.Trait} {R A : Set} (v : A) : Monad R (MutRef A) :=
+  fun fuel s =>
+  RawMonad.AddressOracle (B := A) (fun r =>
+  match r, v with
+  | MutRef.Make a, _ =>
+    match State.read a s with
+    | Some _ => RawMonad.Impossible
+    | None =>
+      let s := State.write a s v in
+      match State.read a s with
+      | None => RawMonad.Impossible
+      | Some _ => RawMonad.Pure (inl (MutRef.Make a), s)
       end
-    | M.Write index v =>
-      match Allocation.get allocation index with
-      | Some address =>
-        M_State.Cast v (fun v =>
-        let s := State.write address s v in
-        M_State.Pure (tt, allocation, s))
-      | None => M_State.Impossible
+    end
+  end).
+
+Definition read `{State.Trait} {R A : Set} (r : Ref A) : Monad R A :=
+  fun fuel s =>
+  match r with
+  | Ref.Immutable v => RawMonad.Pure (inl v, s)
+  | Ref.OfMutRef r =>
+    match r with
+    | MutRef.Make a =>
+      match State.read a s with
+      | None => RawMonad.Impossible
+      | Some v => RawMonad.Pure (inl v, s)
       end
     end
   end.
 
-Module Run.
-  Inductive t {Address A : Set} : M_State Address A -> A -> Prop :=
-  | Pure (v : A) : t (M_State.Pure v) v
-  | Bind {B : Set} (e1 : M_State Address B) (e2 : B -> M_State Address A)
-      (v1 : B) (v2 : A) :
-    t e1 v1 ->
-    t (e2 v1) v2 ->
-    t (M_State.Bind e1 e2) v2
-  | GetAddress (f : Address -> M_State Address A) (address : Address) (v : A) :
-    t (f address) v ->
-    t (M_State.GetAddress f) v
-  | Cast {B : Set} (v : B) (f : B -> M_State Address A) (v' : A) :
-    t (f v) v' ->
-    t (M_State.Cast v f) v'.
-End Run.
+Definition write `{State.Trait} {R A : Set} (r : MutRef A) (v : A) :
+  Monad R unit :=
+  fun fuel s =>
+  match r, v with
+  | MutRef.Make a, _ => RawMonad.Pure (inl tt, State.write a s v)
+  end.
 
 Module Example.
   (** Code for:
@@ -158,44 +162,48 @@ Module Example.
         let mut x = 5;
         let mut y = 10;
         let mut z = 15;
-        let s1 = x + y + z;
+        let mut flag = true;
+        let s1 = y + z;
         
         x = 50;
         y = 100;
         z = 150;
-        let s2 = x + y + z;
+        let s2 = x + y;
         
         return s1 + s2;
       }
   *)
-  Definition main : M Z :=
-    let* x := M.Malloc 5 in
-    let* y := M.Malloc 10 in
-    let* z := M.Malloc 15 in
-    let* v_x := M.Read x in
-    let* v_y := M.Read y in
-    let* v_z := M.Read z in
-    let s1 := v_x + v_y + v_z in
-    let* _ := M.Write x 50 in
-    let* _ := M.Write y 100 in
-    let* _ := M.Write z 150 in
-    let* v_x := M.Read x in
-    let* v_y := M.Read y in
-    let* v_z := M.Read z in
-    let s2 := v_x + v_y + v_z in
-    M.Pure (s1 + s2).
+  Definition main `{State.Trait} : M Z :=
+    let* x := alloc 5 in
+    let* y := alloc 10 in
+    let* z := alloc 15 in
+    let* flag := alloc true in
+    let* v_x := read (Ref.OfMutRef x) in
+    let* v_y := read (Ref.OfMutRef y) in
+    let* v_z := read (Ref.OfMutRef z) in
+    let s1 := v_y + v_z in
+    let* _ := write x 50 in
+    let* _ := write y 100 in
+    let* _ := write z 150 in
+    let* v_x := read (Ref.OfMutRef x) in
+    let* v_y := read (Ref.OfMutRef y) in
+    let* v_z := read (Ref.OfMutRef z) in
+    let s2 := v_x + v_y in
+    pure (s1 + s2).
 
   Module State.
     Record t : Set := {
       x : option Z;
       y : option Z;
       z : option Z;
+      flag : option bool;
     }.
 
     Definition init : t := {|
       x := None;
       y := None;
       z := None;
+      flag := None;
     |}.
   End State.
   Definition State := State.t.
@@ -204,29 +212,42 @@ Module Example.
     Inductive t : Set :=
     | X
     | Y
-    | Z.
+    | Z
+    | Flag.
   End Address.
   Definition Address := Address.t.
 
   Global Instance State_Trait : State.Trait State Address := {
-    get_Set _ := Z;
-    read address state :=
-      match address with
-      | Address.X => state.(State.x)
-      | Address.Y => state.(State.y)
-      | Address.Z => state.(State.z)
+    get_Set a :=
+      match a with
+      | Address.Flag => bool
+      | _ => Z
       end;
-    write address state value :=
-      match address with
-      | Address.X => {| State.x := Some value; State.y := state.(State.y); State.z := state.(State.z) |}
-      | Address.Y => {| State.x := state.(State.x); State.y := Some value; State.z := state.(State.z) |}
-      | Address.Z => {| State.x := state.(State.x); State.y := state.(State.y); State.z := Some value |}
+    read a s :=
+      match a with
+      | Address.X => s.(State.x)
+      | Address.Y => s.(State.y)
+      | Address.Z => s.(State.z)
+      | Address.Flag => s.(State.flag)
+      end;
+    write a s v :=
+      match a, v with
+      | Address.X, _ => s <| State.x := Some v |>
+      | Address.Y, _ => s <| State.y := Some v |>
+      | Address.Z, _ => s <| State.z := Some v |>
+      | Address.Flag, _ => s <| State.flag := Some v |>
       end;
   }.
 
-  Ltac run_malloc a :=
-    eapply Run.GetAddress with (address := a);
-    apply Run.Cast;
+  Ltac run_address_oracle address :=
+    match goal with
+    | |- Run.t (RawMonad.AddressOracle ?f) ?v =>
+      eapply (Run.AddressOracle (MutRef.Make address) f v)
+    end.
+
+  Ltac run_alloc address :=
+    unfold alloc;
+    run_address_oracle address;
     apply Run.Pure.
 
   Definition is_all_allocated (s : State) : Prop :=
@@ -234,30 +255,32 @@ Module Example.
     State.read address s <> None.
 
   Lemma run_main :
-    exists allocation s,
-    Run.t (run_state 1000 [] State.init main) (330, allocation, s) /\
-    is_all_allocated s.
+    exists s,
+    Run.t (main 1000%nat State.init) (inl 175, s) /\
+    is_all_allocated s /\
+    s.(State.flag) = Some true.
   Proof.
-    repeat eexists.
+    eexists.
+    repeat split.
     { unfold main.
       eapply Run.Bind. {
-        run_malloc Address.X.
+        run_alloc Address.X.
       }
       eapply Run.Bind. {
-        run_malloc Address.Y.
+        run_alloc Address.Y.
       }
       eapply Run.Bind. {
-        run_malloc Address.Z.
+        run_alloc Address.Z.
       }
-      repeat (eapply Run.Bind; [
-        apply Run.Cast;
-        apply Run.Pure
-      |]).
+      eapply Run.Bind. {
+        run_alloc Address.Flag.
+      }
+      cbn.
       apply Run.Pure.
     }
-    { simpl.
-      unfold is_all_allocated.
-      now intros [].
+    { unfold is_all_allocated.
+      intros []; discriminate.
     }
+    { reflexivity. }
   Qed.
 End Example.
